last outstanding error - in by_cases

src/locomp-clean.lean
@@ -22,9 +22,9 @@ def vname := string
 
 def val := ℤ
 
-def stack := list ℤ -- TODO: ???val??? how do we make it accept, because +, -, *, / is not defined for val
+def stack := list ℤ 
 
-
+/- ## Reflexive Transitive Closure - Star -/
 namespace rtc
 
 inductive star {α : Sort*} (r : α → α → Prop) (a : α) : α → Prop
@@ -212,21 +212,21 @@ open instr
 def iexec : instr → config → config
 | (LOADI n) (i, s, stk) := (i + 1, s, n :: stk)
 | (LOAD v) (i, s, stk) := (i + 1, s, s v :: stk)
-| ADD (i, s, stk) := (i + 1, s, (head2 stk + stk.head) :: tail2 stk)
-| SUB (i, s, stk) := (i + 1, s, (head2 stk - stk.head) :: tail2 stk)
-| MUL (i, s, stk) := (i + 1, s, (head2 stk * stk.head) :: tail2 stk)
-| DIV (i, s, stk) := (i + 1, s, (head2 stk / stk.head) :: tail2 stk)
+| ADD (i, s, stk) := (i + 1, s, (stk.tail.head + stk.head) :: stk.tail.tail)
+| SUB (i, s, stk) := (i + 1, s, (stk.tail.head - stk.head) :: stk.tail.tail)
+| MUL (i, s, stk) := (i + 1, s, (stk.tail.head * stk.head) :: stk.tail.tail)
+| DIV (i, s, stk) := (i + 1, s, (stk.tail.head / stk.head) :: stk.tail.tail)
 | (STORE v) (i, s, stk) := (i + 1, s{v ↦ (stk.head)}, stk.tail)
 | (JMP n) (i, s, stk) := (i + 1 + n, s, stk)
 | (JMPLESS n) (i, s, stk) := 
-  if (head2 stk) < (stk.head)
-  then (i + 1 + n, s, tail2 stk)
-  else (i + 1, s, tail2 stk)
+  if (stk.tail.head) < (stk.head)
+  then (i + 1 + n, s, stk.tail.tail)
+  else (i + 1, s, stk.tail.tail)
 | (JMPGE n) (i, s, stk) := 
-  if (head2 stk) ≥ (stk.head)
-  then (i + 1 + n, s, tail2 stk)
-  else (i + 1, s, tail2 stk)
-| NOP (i, s, stk) := (i + 1, s, stk)
+  if (stk.tail.head) ≥ (stk.head)
+  then (i + 1 + n, s, stk.tail.tail)
+  else (i + 1, s, stk.tail.tail)
+| NOP (i, s, stk) := (i, s, stk)
 
 /- redefinition for ints rather than nat -/ 
 def nth : list instr → ℤ → instr  
@@ -241,7 +241,7 @@ def nth : list instr → ℤ → instr
   check if pc is in a valid location in the list 
 -/
 def exec1  (li : list instr) (c : config)  (c' : config) : Prop := 
-(∃ i s stk, c = (i, s, stk) ∧ c' = iexec (nth li i) (i, s, stk) ∧ 0 ≤ i ∧ i < li.length)  
+( c' = iexec (nth li c.fst) c ∧ 0 ≤ c.fst ∧ c.fst < li.length)  
 
 /-
 lemma exec1I [intro, code_pred_intro]:
@@ -258,40 +258,12 @@ lemma exec1I {li : list instr} {i s stk c'}
   exec1 li (i, s, stk) c' := 
   begin 
     simp [exec1],
-    use i,
-    use s,
-    use stk,
-    simp [h1, h2, h3]
+    simp [h1, h2, h3],
   end
-
--- lemma exec_trans {li : list instr} {c1 c2 c3 : config}
---   (h1 : exec1 li c1 c2)
---   (h2 : exec1 li c2 c3) :
---   exec1 li c1 c3 :=
---   begin
---     -- Use the definition of exec1 to unpack the assumptions
-
---     rcases h1 with ⟨i1, s1, stk1, hc1, hc2, hi1⟩,
---     rcases h2 with ⟨i2, s2, stk2, hc2', hc3, hi2⟩,
---     -- Use transitivity of execution to relate the two configurations
---     -- subst hc2,
---     have h : i1 < li.length,
---     { linarith [hi1, hi2] },
---     -- Apply exec1I lemma to obtain the transitivity lemma
---     -- exact exec1I hc3 hi1.left h,
---     sorry
---     -- TODO: replace exec1 right side of c3 with h1 items 
---   end
-
-
-
 
 abbreviation exec (li : list instr) (c : config) (c' : config) : Prop :=
 star (exec1 li) c c'
 
-/-
-lemmas exec_induct = star.induct [of "exec1 P", split_format(complete)]
--/
 
 
 -- VERIFICATION INFRASTRUCTURE
@@ -430,14 +402,12 @@ begin
   },
   case NOP {
     simp [iexec],
-    intros h1 h2,
-    apply iexec_shift_without_jmp,
   },
 end
 
 
 @[simp]
-theorem list.zero_le_length {α : Type} (l : list α) : 0 ≤ list.length l :=
+theorem list.length_nneg {α : Type} (l : list α) : 0 ≤ list.length l :=
 begin
   induction l with hd tl hl,
   case list.nil { simp,},
@@ -568,62 +538,41 @@ lemma exec1_appendR {li c c' li'} (h: exec1 li c c'):
 exec1 (li ++ li') c c' :=
 begin
   simp [exec1],
-  obtain ⟨i, s, stk, hi, h_conds⟩ := h,
+  obtain ⟨h_c', h_zero, h_li⟩ := h,
   induction li,
   case list.nil { 
-    use i,
-    use s,
-    use stk,
     unfold_coes, --for int.of_nat in the goal - types
-    split,
-    {
-      apply hi,
-    },
-    simp at h_conds,
     have h_f : false, begin 
-      have h_imore: 0 ≤ i, from h_conds.right.left,
-      have h_iless: i < 0, from  h_conds.right.right,
+      simp at h_li,
       linarith,
     end,
-    apply false.elim,
-    show false, from h_f,
+    cc,    
   },
   case list.cons {
-    by_cases h_izero : (i = 0),
+    by_cases h_izero : (c.fst = 0),
     {
-      use i,
-      use s,
-      use stk,
       simp,
       simp [nth, h_izero] at *,
       split,
-      {apply hi,},
-      split,
-      {apply h_conds,},
-      {linarith,},
+      {apply h_c',},
+      linarith,
     },
     {
-      use i,
-      use s,
-      use stk,
-      have h_inneg : 0 ≤ i, from h_conds.right.left,  
-      have h_ipos : 0 ≤ i - 1, from i_pos h_conds.right.left h_izero, 
-      split,
-      {apply hi,},
+      have h_inneg : 0 ≤ c.fst, from h_zero,  
+      have h_ipos : 0 ≤ c.fst - 1, from i_pos h_zero h_izero, 
       split,
       {
-        clear hi,
-        simp [nth] at h_conds,
-        simp [h_izero] at h_conds,
+        simp [nth] at h_c',
+        simp [h_izero] at h_c',
         simp [nth],
         simp [h_izero],
-        have h_append_eq : nth (li_tl ++ li') (i - 1) = nth li_tl (i - 1) :=
+        have h_append_eq : nth (li_tl ++ li') (c.fst - 1) = nth li_tl (c.fst - 1) :=
         begin 
           rw [nth_append],
           {
-            have h_ite : i - 1 < int.of_nat (list.length li_tl) :=
+            have h_ite : c.fst - 1 < int.of_nat (list.length li_tl) :=
             begin
-              have h_less : i < ↑(list.length li_tl) + 1, from h_conds.right.right,
+              have h_less : c.fst < ↑(list.length li_tl) + 1, from h_li,
               simp,
               linarith,
             end,
@@ -635,17 +584,15 @@ begin
           },
           {exact h_ipos,},
         end,
-        rw h_conds.left,
+        rw h_c',
         rw h_append_eq,
       },
       split,
+      {apply h_inneg,},
       {
-        apply h_conds.right.left,
-      },
-      {
-        have h_length : i < ↑(list.length (li_hd :: li_tl)), from h_conds.right.right,
+        have h_length : c.fst < ↑(list.length (li_hd :: li_tl)), from h_li,
         linarith,
-      },
+      }
     },
   },
 end
@@ -693,108 +640,32 @@ lemma exec1_appendL {i i' :ℤ} {li li' s stk s' stk'}
 (h_li : exec1 li (i, s, stk) (i', s', stk')) :
 exec1 (li' ++ li) ((list.length li') + i, s, stk) ((list.length li') + i', s', stk') :=
 begin
-  induction li' generalizing i,
-  case list.nil {
-    simp,
-    exact h_li,
+  simp [exec1],
+  obtain ⟨ h_c', h_zero, h_length⟩ := h_li,
+  simp at *,
+  have h_li_i : 0 ≤ ↑(list.length li') + i :=
+  begin
+    linarith,
+  end,
+  split,
+  {
+    simp [iexec_shift, nth_append h_li_i],
+    by_cases h_less : (i < 0),
+    {
+      apply false.elim,
+      linarith,
+    },
+    {
+      simp [h_less],
+      apply h_c',
+    }
   },
-  case list.cons {
-    simp [exec1],
-    simp [exec1] at li'_ih,
-    obtain ⟨ih, sh, stkh, hi, h_conds⟩ := h_li,
-    use i,
-    use s,
-    use stk,
-    simp at hi,
-    have h_i : ih = i := 
-    begin symmetry, exact hi.left, end,
-    have h_s : sh = s := 
-    begin symmetry, exact hi.right.left, end,
-    have h_stk : stkh = stk := 
-    begin symmetry, exact hi.right.right, end,
-    rw [h_i] at h_conds,
-    rw [h_s] at h_conds,
-    rw [h_stk] at h_conds,
-    clear h_i,
-    clear h_s,
-    clear h_stk,
-    split,
-    {
-      simp [hi],
-      specialize li'_ih h_conds.left,
-      specialize li'_ih h_conds.right.left,
-      specialize li'_ih h_conds.right.right,
-      -- how to use this: specialize li'_ih h_conds.left,
-      -- how can this ever be true? ↑(list.length li'_tl) + 1 = 0
-      sorry,
-    },
-    {
-      simp [nth],
-      by_cases h_izero : (i = 0),
-      {
-        simp [h_izero],
-        split,
-        {
-          specialize li'_ih h_conds.left,
-
-          specialize li'_ih h_conds.right.left,
-          specialize li'_ih h_conds.right.right,
-          cases li'_ih with i_ih li'_ih_i,
-          cases li'_ih_i with s_ih li'_ih_i_s,
-          cases li'_ih_i_s with stk_ih li'_ih_full,
-          
-          have ih_left : ↑(list.length li'_tl) + i = i_ih ∧ s = s_ih ∧ stk = stk_ih, from li'_ih_full.left,
-          have h_i : i_ih = ↑(list.length li'_tl) + i := 
-            begin symmetry, exact ih_left.left, end,
-          have h_s : s_ih = s := 
-            begin symmetry, exact ih_left.right.left, end,
-          have h_stk : stk_ih = stk := 
-            begin symmetry, exact ih_left.right.right, end,
-          rw [h_i] at li'_ih_full,
-          rw [h_s] at li'_ih_full,
-          rw [h_stk] at li'_ih_full,
-          simp [nth_append] at li'_ih_full,
-
-          simp [h_izero] at h_conds,
-
-          -- maybe iexec shift can be applied here?
-          sorry,
-        },
-        linarith,
-      },
-      {
-        simp [h_izero],
-        split,
-        {
-
-          specialize li'_ih h_conds.left,
-
-          specialize li'_ih h_conds.right.left,
-          specialize li'_ih h_conds.right.right,
-          cases li'_ih with i_ih li'_ih_i,
-          cases li'_ih_i with s_ih li'_ih_i_s,
-          cases li'_ih_i_s with stk_ih li'_ih_full,
-          
-          have ih_left : ↑(list.length li'_tl) + i = i_ih ∧ s = s_ih ∧ stk = stk_ih, from li'_ih_full.left,
-          have h_i : i_ih = ↑(list.length li'_tl) + i := 
-            begin symmetry, exact ih_left.left, end,
-          have h_s : s_ih = s := 
-            begin symmetry, exact ih_left.right.left, end,
-          have h_stk : stk_ih = stk := 
-            begin symmetry, exact ih_left.right.right, end,
-          rw [h_i] at li'_ih_full,
-          rw [h_s] at li'_ih_full,
-          rw [h_stk] at li'_ih_full,
-          simp [nth_append] at li'_ih_full,
-          
-          -- the gap does not seem to easily add up
-          sorry,
-        },
-        split,
-        {apply h_conds.right.left},
-        {linarith,}
-      }
-    },
+  split,
+  {
+    apply h_li_i,
+  },
+  {
+    apply h_length,
   }
 end
 
@@ -806,7 +677,7 @@ lemma exec_appendL:
   P' @ P ⊢ (size(P')+i,s,stk) →* (size(P')+i',s',stk')"
   by (induction rule: exec_induct) (blast intro: star.step exec1_appendL)+
 -/
-lemma exec_appendL {i i' :ℤ} {li li' i s stk i' s' stk'}
+lemma exec_appendL {i i' :ℤ} (li li' i s stk i' s' stk')
 (h_single : exec li (i, s, stk) (i', s', stk')) :
 exec (li' ++ li) (list.length li' + i, s, stk) (list.length li' + i', s', stk') :=
 begin
@@ -815,19 +686,17 @@ begin
     apply rtc.star.refl,
   },
   case LoComp.rtc.star.tail : b hab hbc ih{
-    have h_b : b = (i', s', stk') :=
-    begin
-      sorry,
-    end,
+    specialize ih li' b.fst b.snd.fst b.snd.snd,
+    simp at ih,
     apply rtc.star.tail,
-    {      
-      specialize ih h_b,
-      apply li',
+    {
       apply ih,
     },
     {
+      have h_b : b.snd = (b.snd.fst, b.snd.snd) := by finish,
+      rw [h_b], 
       apply exec1_appendL,
-      simp [h_b] at hbc,
+      simp,
       exact hbc,
     },
   },
@@ -853,9 +722,10 @@ exec (instr :: li) (1, s, stk) (1 + j, t, stk') :=
 begin 
   have h_shift : exec ([instr] ++ li) ((list.length [instr]) + 0, s, stk) ((list.length [instr]) + j, t, stk') :=
   begin 
-    apply exec_appendL h,
+    apply exec_appendL,
     apply j,
     apply j,
+    apply h,
   end,
   simp at h_shift,
   exact h_shift,
@@ -879,9 +749,10 @@ exec (li' ++ li) (i, s, stk) (i', s', stk') :=
 begin
   have h_append : exec (li' ++ li) (list.length li' + (i - list.length li'), s, stk) (list.length li' + j, s', stk') :=
   begin
-    apply exec_appendL h2,
+    apply exec_appendL,
     apply i,
     apply i,
+    apply h2,
   end,
   simp at h_append,
   rw [h3],
@@ -918,9 +789,10 @@ begin
   exact h_appendR_li',
   have h_appendL_li : exec (li ++ li') (list.length li + (i' - list.length li), s', stk') (list.length li + i'', s'', stk'') :=
   begin
-    apply exec_appendL h3,
+    apply exec_appendL,
     apply i',
     apply i',
+    apply h3,
   end,
   simp at h_appendL_li,
   rw [h4],
@@ -928,19 +800,46 @@ begin
 end
 
 /-
-declare Let_def[simp]
+# Compilation
 
 
-subsection "Compilation"
-
+## Arithmetic compilation
 fun acomp :: "aexp ⇒ instr list" where
 "acomp (N n) = [LOADI n]" |
 "acomp (V x) = [LOAD x]" |
 "acomp (Plus a1 a2) = acomp a1 @ acomp a2 @ [ADD]"
 
-lemma acomp_correct[intro]:
-  "acomp a ⊢ (0,s,stk) →* (size(acomp a),s,aval a s#stk)"
-by (induction a arbitrary: stk) fastforce+
+-/
+inductive aexp : Type
+| num : ℤ → aexp
+| var : string → aexp
+| add : aexp → aexp → aexp
+| sub : aexp → aexp → aexp
+| mul : aexp → aexp → aexp
+| div : aexp → aexp → aexp
+
+open aexp
+
+def eval  : aexp → state → ℤ
+| (num i) s    := i
+| (var x) s    := s x
+| (add e₁ e₂) s := eval e₁ s + eval e₂ s
+| (sub e₁ e₂) s := eval e₁ s - eval e₂ s
+| (mul e₁ e₂) s := eval e₁ s * eval e₂ s
+| (div e₁ e₂) s := eval e₁ s / eval e₂ s
+
+
+def acomp : aexp → list instr
+| (num n) := [LOADI n]
+| (var x) := [LOAD x]
+| (add e₁ e₂) := acomp e₁ ++ acomp e₂ ++ [ADD]
+| (sub e₁ e₂) := acomp e₁ ++ acomp e₂ ++ [SUB]
+| (mul e₁ e₂) := acomp e₁ ++ acomp e₂ ++ [MUL]
+| (div e₁ e₂) := acomp e₁ ++ acomp e₂ ++ [DIV]
+
+
+/-
+## Boolean compilation
 
 fun bcomp :: "bexp ⇒ bool ⇒ int ⇒ instr list" where
 "bcomp (Bc v) f n = (if v=f then [JMP n] else [])" |
@@ -956,23 +855,33 @@ fun bcomp :: "bexp ⇒ bool ⇒ int ⇒ instr list" where
 value
   "bcomp (And (Less (V ''x'') (V ''y'')) (Not(Less (V ''u'') (V ''v''))))
      False 3"
+-/
+inductive bexp : Type
+| Bc : Prop → bexp
+| Not : bexp → bexp
+| And : bexp → bexp → bexp
+| Less : aexp → aexp → bexp
 
-lemma bcomp_correct[intro]:
-  fixes n :: int
-  shows
-  "0 ≤ n ⟹
-  bcomp b f n ⊢
- (0,s,stk)  →*  (size(bcomp b f n) + (if f = bval b s then n else 0),s,stk)"
-proof(induction b arbitrary: f n)
-  case Not
-  from Not(1)[where f="~f"] Not(2) show ?case by fastforce
-next
-  case (And b1 b2)
-  from And(1)[of "if f then size(bcomp b2 f n) else size(bcomp b2 f n) + n" 
-                 "False"] 
-       And(2)[of n f] And(3) 
-  show ?case by fastforce
-qed fastforce+
+open bexp
+def bval : bexp → state → Prop
+| (Bc v) s    := v
+| (Not b) s   := ¬(bval b s)
+| (And b1 b2) s := bval b1 s ∧ bval b2 s
+| (Less a1 a2) s := (eval a1 s) < (eval a2 s) 
+
+noncomputable def bcomp : bexp → Prop → ℤ → list instr  --TODO: TD6: find out whether noncomputable is okay
+| (Bc v) f n := if (v = f) then [JMP n] else []
+| (Not b) f n :=  bcomp b (¬ f) n
+| (And b1 b2) f n := 
+    let cb2 := bcomp b2 f n,
+      m := if (f = true) then int.of_nat (list.length cb2) else int.of_nat (list.length cb2) + n,
+      cb1 := bcomp b1 false m
+    in cb1 ++ cb2
+| (Less a1 a2) f n := acomp a1 ++ acomp a2 ++ 
+  (if (f = true) then [JMPLESS n] else [JMPGE n])
+
+/-
+## Command compilation
 
 fun ccomp :: "com ⇒ instr list" where
 "ccomp SKIP = []" |
@@ -991,9 +900,661 @@ value "ccomp
   ELSE ''v'' ::= V ''u'')"
 
 value "ccomp (WHILE Less (V ''u'') (N 1) DO (''u'' ::= Plus (V ''u'') (N 1)))"
+-/
+
+inductive com : Type
+| SKIP : com
+| Assign : vname → aexp → com
+| Seq : com → com → com
+| If : bexp → com → com → com
+| While : bexp → com → com
+
+open com
+
+noncomputable def ccomp : com → list instr
+| com.SKIP := []
+| (Assign x a) := acomp a ++ [STORE x]
+| (Seq c1 c2) := ccomp c1 ++ ccomp c2
+| (If b c1 c2) := (
+  let cc1 := ccomp c1,
+    cc2 := ccomp c2,
+    cb := bcomp b false (list.length cc1 + 1)
+  in cb ++ cc1 ++ (JMP (list.length cc2) :: cc2)
+)
+| (While b c) := (
+  let cc := ccomp c,
+    cb := bcomp b false (list.length cc + 1)
+  in cb ++ cc ++ [JMP (-(list.length cb + list.length cc + 1))] 
+)
+open com
+
+infixr ` ;; ` : 90 := Seq
+
+def silly_loop {s : state} : com :=
+While ( Bc ( s "x" > s "y") )
+  (SKIP ;; Assign "x" (num ((s "x") - 1)))
 
 
-subsection "Preservation of semantics"
+inductive big_step : com × state → state → Prop
+| skip {s} :
+  big_step (SKIP, s) s
+| assign {x a s} :
+  big_step (Assign x a, s) (s{x ↦ eval a s})
+| seq {S T s t u} (hS : big_step (S, s) t)
+    (hT : big_step (T, t) u) :
+  big_step (S ;; T, s) u
+| ite_true {b : bexp} {S T s t} (hcond : bval b s)
+    (hbody : big_step (S, s) t) :
+  big_step (com.If b S T, s) t
+| ite_false {b : bexp} {S T s t} (hcond : ¬bval b s)
+    (hbody : big_step (T, s) t) :
+  big_step (com.If b S T, s) t
+| while_true {b : bexp} {S s t u} (hcond : bval b s)
+    (hbody : big_step (S, s) t)
+    (hrest : big_step (While b S, t) u) :
+  big_step (While b S, s) u
+| while_false {b : bexp} {S s} (hcond : ¬ bval b s) :
+  big_step (While b S, s) s
+
+infix ` ⟹ ` : 110 := big_step
+
+
+/-! ## Properties of the Big-Step Semantics
+
+Equipped with a big-step semantics, we can
+
+* prove properties of the programming language, such as **equivalence proofs**
+  between programs and **determinism**;
+
+* reason about **concrete programs**, proving theorems relating final states `t`
+  with initial states `s`. -/
+
+lemma big_step_deterministic {S s l r} (hl : (S, s) ⟹ l)
+    (hr : (S, s) ⟹ r) :
+  l = r :=
+begin
+  induction' hl,
+  case skip {
+    cases' hr,
+    refl },
+  case assign {
+    cases' hr,
+    refl },
+  case seq : S T s t l hS hT ihS ihT {
+    cases' hr with _ _ _ _ _ _ _ t' _ hS' hT',
+    cases' ihS hS',
+    cases' ihT hT',
+    refl },
+  case ite_true : b S T s t hb hS ih {
+    cases' hr,
+    { apply ih hr },
+    { cc } },
+  case ite_false : b S T s t hb hT ih {
+    cases' hr,
+    { cc },
+    { apply ih hr } },
+  case while_true : b S s t u hb hS hw ihS ihw {
+    cases' hr,
+    { cases' ihS hr,
+      cases' ihw hr_1,
+      refl },
+    { cc } },
+  { cases' hr,
+    { cc },
+    { refl } }
+end
+
+-- lemma big_step_terminates {S s} :
+--   ∃t, (S, s) ⟹ t :=
+-- sorry   -- unprovable
+
+lemma big_step_doesnt_terminate {S s t} :
+  ¬ (While (Bc ( true)) S, s) ⟹ t :=
+begin
+  intro hw,
+  induction' hw,
+  case while_true {
+    assumption },
+  case while_false {
+    simp [bval] at hcond,
+    cc }
+end
+
+/-! We can define inversion rules about the big-step semantics: -/
+
+@[simp] lemma big_step_skip_iff {s t} :
+  (SKIP, s) ⟹ t ↔ t = s :=
+begin
+  apply iff.intro,
+  { intro h,
+    cases' h,
+    refl },
+  { intro h,
+    rw h,
+    exact big_step.skip }
+end
+
+@[simp] lemma big_step_assign_iff {x a s t} :
+  (Assign x a, s) ⟹ t ↔ t = s{x ↦ eval a s} :=
+begin
+  apply iff.intro,
+  { intro h,
+    cases' h,
+    refl },
+  { intro h,
+    rw h,
+    exact big_step.assign }
+end
+
+@[simp] lemma big_step_seq_iff {S T s t} :
+  (S ;; T, s) ⟹ t ↔ (∃u, (S, s) ⟹ u ∧ (T, u) ⟹ t) :=
+begin
+  apply iff.intro,
+  { intro h,
+    cases' h,
+    apply exists.intro,
+    apply and.intro; assumption },
+  { intro h,
+    cases' h,
+    cases' h,
+    apply big_step.seq; assumption }
+end
+
+@[simp] lemma big_step_ite_iff {b S T s t} :
+  (com.If b S T, s) ⟹ t ↔
+  (bval b s ∧ (S, s) ⟹ t) ∨ (¬ bval b s ∧ (T, s) ⟹ t) :=
+begin
+  apply iff.intro,
+  { intro h,
+    cases' h,
+    { apply or.intro_left,
+      cc },
+    { apply or.intro_right,
+      cc } },
+  { intro h,
+    cases' h; cases' h,
+    { apply big_step.ite_true; assumption },
+    { apply big_step.ite_false; assumption } }
+end
+
+lemma big_step_while_iff {b S s u} :
+  (While b S, s) ⟹ u ↔
+  (∃t, bval b s ∧ (S, s) ⟹ t ∧ (While b S, t) ⟹ u)
+  ∨ (¬ bval b s ∧ u = s) :=
+begin
+  apply iff.intro,
+  { intro h,
+    cases' h,
+    { apply or.intro_left,
+      apply exists.intro t,
+      cc },
+    { apply or.intro_right,
+      cc } },
+  { intro h,
+    cases' h,
+    case inl {
+      cases' h with t h,
+      cases' h with hb h,
+      cases' h with hS hwhile,
+      exact big_step.while_true hb hS hwhile },
+    case inr {
+      cases' h with hb hus,
+      rw hus,
+      exact big_step.while_false hb } }
+end
+
+lemma big_step_while_true_iff {b : bexp} {S s u}
+    (hcond : bval b s) :
+  (While b S, s) ⟹ u ↔
+  (∃t, (S, s) ⟹ t ∧ (While b S, t) ⟹ u) :=
+by rw big_step_while_iff; simp [hcond]
+
+@[simp] lemma big_step_while_false_iff {b : bexp}
+    {S s t} (hcond : ¬ bval b s) :
+  (While b S, s) ⟹ t ↔ t = s :=
+by rw big_step_while_iff; simp [hcond]
+
+
+/-
+
+# Compilation correctness
+
+## acomp correctness
+lemma acomp_correct[intro]:
+  "acomp a ⊢ (0,s,stk) →* (size(acomp a),s,aval a s#stk)"
+by (induction a arbitrary: stk) fastforce+
+
+-/
+
+lemma acomp_correct {a : aexp}  {s : state}  {stk : stack} :
+exec (acomp a) (0, s, stk) (list.length (acomp a), s, (eval a s) :: stk) :=
+begin
+  induction a generalizing stk,
+  case num {  --DONE
+    simp [acomp, eval],
+    apply rtc.star.single,
+    apply exec1I,
+    {
+      simp [nth],
+      simp[iexec],
+    },
+    {
+      linarith,
+    },
+    {
+      simp,
+    }
+  },
+  case var {  --DONE
+    simp [acomp, eval],
+    apply rtc.star.single,
+    apply exec1I,
+    {
+      simp [nth],
+      simp[iexec],
+    },
+    {
+      linarith,
+    },
+    {
+      simp,
+    }
+  },
+  case add : a b a_i b_i{ --DONE
+    simp [acomp],
+    --trans a ++ (b ++ [OP])
+    apply exec_append_trans,
+    apply int.of_nat(list.length (acomp a)),
+    exact a_i,
+    simp,
+    {
+      have h_b_add : exec (acomp b ++ [ADD]) (↑(list.length (acomp a)) - ↑(list.length (acomp a)), s, eval a s :: stk) (list.length (acomp b) + 1, s, eval (add a b) s :: stk) := 
+      begin
+        simp,
+        --trans b ++ [OP]
+        apply exec_append_trans,
+        apply int.of_nat(list.length (acomp b)),
+        exact b_i,
+        simp,
+        {
+          simp,
+          have h_add: exec [ADD] (0, s, eval b s :: eval a s :: stk) (1, s, eval (add a b) s :: stk) := 
+          begin
+            apply rtc.star.single,
+            apply exec1I,
+            {
+              simp [nth, iexec, eval],
+            },
+            linarith,
+            simp,
+          end,
+          exact h_add,
+        },
+        refl,
+      end,
+      exact h_b_add,
+    },
+    refl,
+  },
+  case sub : a b a_i b_i{ --DONE
+    simp [acomp],
+    --trans a ++ (b ++ [OP])
+    apply exec_append_trans,
+    apply int.of_nat(list.length (acomp a)),
+    exact a_i,
+    simp,
+    {
+      have h_b_add : exec (acomp b ++ [SUB]) (↑(list.length (acomp a)) - ↑(list.length (acomp a)), s, eval a s :: stk) (list.length (acomp b) + 1, s, eval (sub a b) s :: stk) := 
+      begin
+        simp,
+        --trans b ++ [OP]
+        apply exec_append_trans,
+        apply int.of_nat(list.length (acomp b)),
+        exact b_i,
+        simp,
+        {
+          simp,
+          have h_add: exec [SUB] (0, s, eval b s :: eval a s :: stk) (1, s, eval (sub a b) s :: stk) := 
+          begin
+            apply rtc.star.single,
+            apply exec1I,
+            {
+              simp [nth, iexec, eval],
+            },
+            linarith,
+            simp,
+          end,
+          exact h_add,
+        },
+        refl,
+      end,
+      exact h_b_add,
+    },
+    refl,
+  },
+  case mul : a b a_i b_i{ --DONE
+    simp [acomp],
+    --trans a ++ (b ++ [OP])
+    apply exec_append_trans,
+    apply int.of_nat(list.length (acomp a)),
+    exact a_i,
+    simp,
+    {
+      have h_b_add : exec (acomp b ++ [MUL]) (↑(list.length (acomp a)) - ↑(list.length (acomp a)), s, eval a s :: stk) (list.length (acomp b) + 1, s, eval (mul a b) s :: stk) := 
+      begin
+        simp,
+        --trans b ++ [OP]
+        apply exec_append_trans,
+        apply int.of_nat(list.length (acomp b)),
+        exact b_i,
+        simp,
+        {
+          simp,
+          have h_add: exec [MUL] (0, s, eval b s :: eval a s :: stk) (1, s, eval (mul a b) s :: stk) := 
+          begin
+            apply rtc.star.single,
+            apply exec1I,
+            {
+              simp [nth, iexec, eval],
+            },
+            linarith,
+            simp,
+          end,
+          exact h_add,
+        },
+        refl,
+      end,
+      exact h_b_add,
+    },
+    refl,
+  },
+  case div : a b a_i b_i{ --DONE
+    simp [acomp],
+    --trans a ++ (b ++ [OP])
+    apply exec_append_trans,
+    apply int.of_nat(list.length (acomp a)),
+    exact a_i,
+    simp,
+    {
+      have h_b_add : exec (acomp b ++ [DIV]) (↑(list.length (acomp a)) - ↑(list.length (acomp a)), s, eval a s :: stk) (list.length (acomp b) + 1, s, eval (div a b) s :: stk) := 
+      begin
+        simp,
+        --trans b ++ [OP]
+        apply exec_append_trans,
+        apply int.of_nat(list.length (acomp b)),
+        exact b_i,
+        simp,
+        {
+          simp,
+          have h_add: exec [DIV] (0, s, eval b s :: eval a s :: stk) (1, s, eval (div a b) s :: stk) := 
+          begin
+            apply rtc.star.single,
+            apply exec1I,
+            {
+              simp [nth, iexec, eval],
+            },
+            linarith,
+            simp,
+          end,
+          exact h_add,
+        },
+        refl,
+      end,
+      exact h_b_add,
+    },
+    refl,
+  
+  },
+
+end
+
+
+/-
+
+## bcomp correctness
+lemma bcomp_correct[intro]:
+  fixes n :: int
+  shows
+  "0 ≤ n ⟹
+  bcomp b f n ⊢
+ (0,s,stk)  →*  (size(bcomp b f n) + (if f = bval b s then n else 0),s,stk)"
+proof(induction b arbitrary: f n)
+  case Not
+  from Not(1)[where f="~f"] Not(2) show ?case by fastforce
+next
+  case (And b1 b2)
+  from And(1)[of "if f then size(bcomp b2 f n) else size(bcomp b2 f n) + n" 
+                 "False"] 
+       And(2)[of n f] And(3) 
+  show ?case by fastforce
+qed fastforce+
+-/
+
+lemma not_not_eq {α β : Prop}
+(h_not_eq : ¬ (α = β)) :
+α = ¬ β :=
+begin
+  rw [eq_iff_iff] at *,
+  rw [not_iff] at h_not_eq,
+  apply iff.not_right,
+  exact h_not_eq,
+end
+
+lemma bcomp_correct (n: ℤ) ( b f s stk)
+(h_nneg : 0 ≤  n) :
+exec (bcomp b f n) (0, s, stk) (list.length (bcomp b f n) + (if (f = bval b s) then n else 0), s, stk) :=
+begin
+  induction b generalizing f n,
+  case Bc { --DONE
+    simp [bcomp],
+    rw [bval],
+    by_cases h_b_is_f : (b = f),
+    {
+      simp [h_b_is_f],
+      apply rtc.star.single,
+      apply exec1I,
+      {simp [nth],simp[iexec],},
+      {linarith,},
+      {simp,}
+    },
+    {
+      simp [h_b_is_f],
+      have h_fnotb : ¬ f = b := by cc, 
+      simp [h_fnotb],
+      apply rtc.star.refl,
+    }
+  },
+  case Not : b{ --DONE
+    specialize b_ih (¬f) n,
+    -- apply rtc.star.single,
+    simp [bcomp],
+    rw [bval],
+    by_cases h_bisf : (f = bval b s),
+    {
+      simp [h_bisf],
+      rw [h_bisf] at b_ih,
+      simp * at b_ih,
+      exact b_ih,
+    },
+    {
+      have h_fneg : f = ¬ bval b s := 
+      begin
+        apply not_not_eq,
+        exact h_bisf,
+      end,
+      simp [h_fneg],
+      rw [h_fneg] at b_ih,
+      simp * at b_ih,
+      exact b_ih,
+    }
+  },
+  case And : b1 b2 ih1 ih2{ --INCOMPLETE: error: occurs check failed.
+
+    simp [bcomp, bval],
+    by_cases h_f : (f = true),
+    {
+      simp [h_f],
+      rw [bval],
+      apply exec_append_trans,
+      apply int.of_nat ((bcomp b1 false ↑((bcomp b2 true n).length)).length),
+      {
+        specialize ih1 false (int.of_nat (list.length (bcomp b2 f n))),
+        simp at ih1,
+        simp [h_f] at ih1,
+        apply ih1,
+      },
+      simp,
+      {
+        by_cases h_b1 : (false = bval b1 s),
+        simp [h_b1],
+        simp [h_b1],
+      },
+      {
+        simp,
+        specialize ih2 true n,
+        simp [h_nneg] at ih2,
+
+        have h_bcomp2 : exec (bcomp b2 true n) (↑((bcomp b2 true n).length), s, stk) (↑((bcomp b2 true n).length), s, stk) :=
+        begin
+          apply rtc.star.refl,
+        end,
+        by_cases h_b1 : (false = bval b1 s),
+        {
+          simp [h_b1],
+          -- length bcomp b2 - apply h_bcomp2
+          apply h_bcomp2,
+        },
+        {
+          simp [h_b1],
+          -- 0 - apply ih2
+          apply ih2,
+        },
+      },
+      finish,
+    },
+    {
+      simp [h_f],
+      rw [bval],
+      have h_imp_nneg : 0 ≤ ↑((bcomp b2 f n).length) + n := 
+      begin
+        have h_list_nneg : 0 ≤ ↑((bcomp b2 f n).length) :=
+        begin
+          simp [list.length_nneg],
+        end,
+        linarith,
+      end,
+      apply exec_append_trans,
+      apply int.of_nat ((bcomp b1 false (↑((bcomp b2 f n).length) + n)).length),
+      {
+        specialize ih1 false (int.of_nat (list.length (bcomp b2 f n)) + n),
+        simp at ih1,        
+        simp [h_imp_nneg] at ih1,
+        apply ih1,
+      },
+      simp,
+      {
+        by_cases h_b1 : (false = bval b1 s),
+        {
+          simp [h_b1],
+          simp [h_imp_nneg],
+        },
+        simp [h_b1],
+      },
+      {
+        simp,
+        specialize ih2 f n,
+        simp [h_nneg] at ih2,
+        have h_bcomp2 : exec (bcomp b2 f n) (↑((bcomp b2 f n).length) + n, s, stk) (↑((bcomp b2 f n).length) + n, s, stk) :=
+        begin
+          apply rtc.star.refl,
+        end,
+        by_cases h_b1 : (false = bval b1 s),
+        {
+          simp [h_b1],
+          apply h_bcomp2,
+        },
+        {
+          simp [h_b1],
+          -- 0 - apply ih2
+          apply ih2,
+        },
+      },
+      simp,
+    },
+  },
+  case Less : a1 a2{  --DONE
+    simp [bcomp],
+    rw [bval],
+    -- acomp a1 ++ (acomp a2 ++ ite (f = true) [JMPLESS n] [JMPGE n])
+    apply exec_append_trans,
+    apply int.of_nat (list.length (acomp a1)),
+    apply acomp_correct,
+    simp,
+    {
+      simp,
+      have h_a2_ite : exec (acomp a2 ++ ite (f = true) [JMPLESS n] [JMPGE n]) (0, s, eval a1 s :: stk) ((↑(list.length (acomp a2)) + ↑(list.length (ite (f = true) [JMPLESS n] [JMPGE n]))) +
+        ite (f = (eval a1 s < eval a2 s)) n 0, s, stk) := 
+      begin
+        -- (acomp a2 ++ ite (f = true) [JMPLESS n] [JMPGE n])
+        apply exec_append_trans,
+        apply int.of_nat (list.length (acomp a2)),
+        apply acomp_correct,
+        simp,
+        {
+          simp,
+          have h_ite : exec (ite (f = true) [JMPLESS n] [JMPGE n]) (0, s, eval a2 s :: eval a1 s :: stk) (↑(list.length (ite (f = true) [JMPLESS n] [JMPGE n])) + ite (f = (eval a1 s < eval a2 s)) n 0, s, stk) := 
+          begin
+            by_cases h_f : (f = true),
+            { -- [JMPLESS]
+              simp [h_f],
+              apply rtc.star.single,
+              apply exec1I,
+              {
+                simp [nth],
+                simp [iexec],
+                by_cases h_ite : (eval a1 s < eval a2 s),
+                {simp [h_ite],},
+                {simp [h_ite],}
+              },
+              simp,
+              simp,
+            },
+            { -- [JMPGE]
+              simp [h_f],
+              apply rtc.star.single,
+              apply exec1I,
+              {
+                simp [nth],
+                simp [iexec],
+                have h_f_false : f = ¬ true :=
+                begin
+                  apply not_not_eq,
+                  exact h_f,
+                end,
+                simp [h_f_false],
+                by_cases h_ite : (eval a2 s ≤ eval a1 s),
+                {simp [h_ite],},
+                {simp [h_ite],}
+              },
+              simp,
+              simp,
+            },
+          end,
+          exact h_ite,
+        },
+        finish,
+      end,
+      exact h_a2_ite,
+    },
+    finish,
+  }
+
+end
+
+
+/-
+
+## Preservation of semantics
 
 lemma ccomp_bigstep:
   "(c,s) ⇒ t ⟹ ccomp c ⊢ (0,s,stk) →* (size(ccomp c),t,stk)"
@@ -1028,8 +1589,270 @@ next
 qed fastforce+
 
 end
-
 -/
+
+
+lemma ccomp_bigstep {c : com} { s : state } {t : state } (stk : stack) 
+(h_step : (c, s) ⟹ t) :
+exec (ccomp c) (0, s, stk) (list.length (ccomp c), t, stk) :=
+begin
+  induction' h_step,
+  case skip { -- DONE
+    simp [ccomp],
+    apply rtc.star.refl,
+  },
+  case assign { -- DONE
+    simp [ccomp],
+    apply exec_append_trans,
+    apply int.of_nat (list.length (acomp a)),
+    apply acomp_correct,
+    simp,
+    {
+      simp,
+      have h_store : exec [STORE x] (0, t, eval a t :: stk) (int.of_nat (list.length ([STORE])), t{x ↦ eval a t}, stk) :=
+      begin
+        apply rtc.star.single,
+        apply exec1I,
+        {
+          simp [nth],
+          simp [iexec],
+        },
+        {simp,},
+        {simp,}
+      end,
+      exact h_store,
+    },
+    simp,
+  },
+  case seq : c1 c2 s u t{ -- DONE
+    simp [ccomp],
+    apply exec_append_trans,
+    apply int.of_nat ((ccomp c1).length),
+    apply ih_h_step,
+    simp,
+    {
+      simp,
+      apply ih_h_step_1,
+    },
+    simp,
+  },
+  case ite_true : b c1 c2 { --DONE
+    simp [ccomp],
+      apply exec_append_trans,
+      apply int.of_nat (bcomp b false (↑((ccomp c1).length) + 1)).length,
+      {
+        have h_bcomp : exec (bcomp (b) (false) (↑((ccomp c1).length) + 1)) (0, s, stk) (↑ ((bcomp (b) (false) (↑((ccomp c1).length) + 1)).length) + ite (false = bval b s) (↑((ccomp c1).length) + 1) 0 , s, stk) :=
+        begin
+          apply bcomp_correct,
+          linarith,
+        end,
+        apply h_bcomp,
+      },
+      simp,
+      {simp [hcond],},
+      {
+        simp,
+        simp [hcond],
+        have h_ccomp_jmp : exec (ccomp c1 ++ JMP ↑((ccomp c2).length) :: ccomp c2) (0, s, stk) (↑((ccomp c1).length) + (↑((ccomp c2).length) + 1), t, stk) := 
+        begin
+          apply exec_append_trans,
+          apply int.of_nat ((ccomp c1).length),
+          apply ih,
+          simp,
+          {
+            simp,
+            have h_jmp_c2 : exec (JMP ↑((ccomp c2).length) :: ccomp c2) (0, t, stk) (↑((ccomp c2).length) + 1, t, stk) :=
+            begin
+              apply rtc.star.single,
+              simp [exec1, nth],
+              simp [iexec],
+              finish, 
+            end,
+            apply h_jmp_c2,
+          },
+          simp,
+        end,
+        apply h_ccomp_jmp,
+      },
+      simp,
+
+  },
+  case ite_false : b c1 c2 { -- DONE
+    simp [ccomp],
+
+    apply exec_append_trans,
+    apply int.of_nat (bcomp b false (↑((ccomp c1).length) + 1)).length,
+    {
+      have h_bcomp : exec (bcomp (b) (false) (↑((ccomp c1).length) + 1)) (0, s, stk) (↑ ((bcomp (b) (false) (↑((ccomp c1).length) + 1)).length) + ite (false = bval b s) (↑((ccomp c1).length) + 1) 0 , s, stk) :=
+      begin
+        apply bcomp_correct,
+        linarith,
+      end,
+      apply h_bcomp,  
+    },
+    simp,
+    {
+      simp [hcond],
+      linarith,
+    },
+    {
+      simp,
+      simp [hcond],
+      have h_ccomp_jmp : exec (ccomp c1 ++ JMP ↑((ccomp c2).length) :: ccomp c2) (↑((ccomp c1).length) + 1, s, stk) (↑((ccomp c1).length) + (↑((ccomp c2).length) + 1), t, stk) := 
+      begin
+        apply exec_appendL_if,
+        simp,
+        {
+          simp,
+          apply exec_cons_1,
+          apply ih,
+        },
+        simp,
+        finish,
+      end,
+      apply h_ccomp_jmp,
+    },
+    simp,
+  },
+  case while_true : b c s1 s2 s3{ --DONE
+    let cc := ccomp c,
+    let cb := bcomp b false (list.length cc + 1),
+    let cw := ccomp(While b c),
+    have h_cond : exec cw (0, s1, stk) (list.length cb, s1, stk) := 
+      begin
+        -- specialize ih_h_step stk,
+        simp [cw, ccomp],
+        simp [cb, cc],
+        apply exec_appendR,
+        have h_with_ite : exec (bcomp b false (↑((ccomp c).length) + 1)) (0, s1, stk)
+          (↑((bcomp b false (↑((ccomp c).length) + 1)).length), s1, stk) =
+          exec (bcomp b false (↑((ccomp c).length) + 1)) (0, s1, stk) 
+          (↑((bcomp b false (↑((ccomp c).length) + 1)).length) + ite (false = bval b s1) (↑((ccomp c).length) + 1) 0, s1, stk) := 
+          begin
+            simp [hcond],
+          end,
+        rw [h_with_ite],
+        apply bcomp_correct,
+        have h_nneg : 0 ≤ ↑((ccomp c).length) :=
+        begin
+          simp [list.length_nneg],
+        end,
+        linarith,
+      end,
+    have h_do : exec cw (list.length cb, s1, stk) (list.length cb + list.length cc, s2, stk) := 
+      begin
+        specialize ih_h_step stk,
+        simp [cw, ccomp],
+        simp [cb, cc],
+        have h_with_zero : exec
+          (bcomp b false (↑((ccomp c).length) + 1) ++
+            (ccomp c ++ [JMP (-1 + (-↑((ccomp c).length) + -↑((bcomp b false (↑((ccomp c).length) + 1)).length)))]))
+          (↑((bcomp b false (↑((ccomp c).length) + 1)).length), s1, stk)
+          (↑((bcomp b false (↑((ccomp c).length) + 1)).length) + ↑((ccomp c).length), s2, stk) =
+          exec
+          (bcomp b false (↑((ccomp c).length) + 1) ++
+            (ccomp c ++ [JMP (-1 + (-↑((ccomp c).length) + -↑((bcomp b false (↑((ccomp c).length) + 1)).length)))]))
+          (↑((bcomp b false (↑((ccomp c).length) + 1)).length) + 0, s1, stk)
+          (↑((bcomp b false (↑((ccomp c).length) + 1)).length) + ↑((ccomp c).length), s2, stk) := by simp,
+        rw [h_with_zero],
+        clear h_with_zero,
+        apply exec_appendL,
+        apply int.of_nat((ccomp c).length),
+        apply int.of_nat((ccomp c).length),
+        apply exec_appendR,
+        apply ih_h_step,
+      end,
+    have h_back : exec cw (list.length cb + list.length cc, s2, stk) (0, s2, stk) := 
+      begin
+        simp [cw, ccomp],
+        simp [cb, cc],
+        have h_with_zero :
+          exec
+          (bcomp b false (↑((ccomp c).length) + 1) ++
+          (ccomp c ++ [JMP (-1 + (-↑((ccomp c).length) + -↑((bcomp b false (↑((ccomp c).length) + 1)).length)))]))
+          (↑((bcomp b false (↑((ccomp c).length) + 1)).length) + ↑((ccomp c).length), s2, stk)
+          (0, s2, stk) =
+          exec
+          (bcomp b false (↑((ccomp c).length) + 1) ++
+          (ccomp c ++ [JMP (-1 + (-↑((ccomp c).length) + -↑((bcomp b false (↑((ccomp c).length) + 1)).length)))]))
+          (↑((bcomp b false (↑((ccomp c).length) + 1)).length) + ↑((ccomp c).length), s2, stk)
+          (↑((bcomp b false (↑((ccomp c).length) + 1)).length) + (↑((ccomp c).length) -↑((bcomp b false (↑((ccomp c).length) + 1)).length) - ↑((ccomp c).length)), s2, stk) := by simp,
+        rw [h_with_zero],
+        clear h_with_zero,
+        apply exec_appendL,
+        apply int.of_nat((ccomp c).length),
+        apply int.of_nat((ccomp c).length),
+        have h_with_zero_2 :
+          exec
+          (ccomp c ++ [JMP (-1 + (-↑((ccomp c).length) + -↑((bcomp b false (↑((ccomp c).length) + 1)).length)))])
+          (↑((ccomp c).length), s2, stk)
+          (↑((ccomp c).length) - ↑((bcomp b false (↑((ccomp c).length) + 1)).length) - ↑((ccomp c).length), s2, stk) =
+         exec
+          (ccomp c ++ [JMP (-1 + (-↑((ccomp c).length) + -↑((bcomp b false (↑((ccomp c).length) + 1)).length)))])
+          (↑((ccomp c).length) + 0, s2, stk)
+          (↑((ccomp c).length)  + ( -↑((bcomp b false (↑((ccomp c).length) + 1)).length)  + -↑((ccomp c).length)), s2, stk) := by simp,
+        rw [h_with_zero_2],
+        clear h_with_zero_2,
+        apply exec_appendL,
+        apply int.of_nat(list.length ([JMP])),
+        apply int.of_nat(list.length ([JMP])),
+        apply rtc.star.single,
+        simp [exec1, nth],
+        simp [iexec],
+        finish,
+      end,
+    have h_out : exec cw (0, s2, stk) (list.length cw, s3, stk) := 
+      begin
+        specialize ih_h_step_1 stk,
+        simp [cw],
+        apply ih_h_step_1,
+      end,
+
+    show exec cw (0,s1,stk) (list.length cw, s3, stk),
+    apply rtc.star.trans,
+    apply h_cond,
+    {
+      apply rtc.star.trans,
+      apply h_do,
+      {
+        apply rtc.star.trans,
+        apply h_back,
+        apply h_out,
+      }
+    },
+  },
+  case while_false : b c{ --DONE
+    let cc := ccomp c,
+    let cb := bcomp b false (list.length cc + 1),
+    let cw := ccomp(While b c),
+    simp [ccomp],
+    apply exec_append_trans,
+    apply int.of_nat (cb.length),
+    {
+        have h_bcomp : exec (bcomp b (false) (↑((ccomp c).length) + 1)) (0, t, stk) (↑ ((bcomp (b) (false) (↑((ccomp c).length) + 1)).length) + ite (false = bval b t) (↑((ccomp c).length) + 1) 0 , t, stk) :=
+        begin
+          apply bcomp_correct,
+          linarith,
+        end,
+        apply h_bcomp, 
+    },
+    {
+      simp [hcond],
+      linarith,
+    },
+    {
+      simp,
+      simp [hcond],
+      have h_ccomp_jmp : exec (ccomp c ++ [JMP (-1 + (-↑((ccomp c).length) + -↑((bcomp b false (↑((ccomp c).length) + 1)).length)))])
+        (↑((ccomp c).length) + 1, t, stk)
+        (↑((ccomp c).length) + 1, t, stk) := 
+        begin apply rtc.star.refl, end,
+      apply h_ccomp_jmp,
+    },
+    simp,
+  },
+end
+
 
 
 end LoComp
